Progress in cwp.v Reduced fair_coin proof to convergence of geometric series and one admitted fact about geometric series. The general cwp <-> compile+inference proof is down to the sequence and while cases.

theory/cwp/cwp.v
@@ -37,11 +37,11 @@ Inductive cpGCL : Type :=
 
 Record prog :=
   { prog_com : cpGCL
-  ; prog_query : exp
-  }.
+  ; prog_query : exp }.
 
 Notation "a ';;' b" := (CSeq a b) (at level 100, right associativity) : cpGCL_scope.
 Open Scope cpGCL_scope.
+Open Scope order_scope.
 
 
 (** Choice trees with fix (loop) nodes *)
@@ -75,12 +75,23 @@ Instance Monad_tree : Monad tree := { ret := Leaf; bind := @tree_bind }.
 Definition kcomp {A B C : Type} (f : A -> tree B) (g : B -> tree C) : A -> tree C :=
   fun x => bind (f x) g.
 
+Inductive wf_tree {A : Type} : tree A -> Prop :=
+| wf_leaf : forall x, wf_tree (Leaf x)
+| wf_fail : forall n, wf_tree (Fail _ n)
+| wf_choice : forall p t1 t2,
+    0 <= p <= 1 ->
+    wf_tree t1 -> wf_tree t2 ->
+    wf_tree (Choice p t1 t2)
+| wf_fix : forall k,
+    (forall n, wf_tree (k n)) ->
+    wf_tree (Fix k).
+
 
 (** Compiling cpGCL commands to trees *)
 Fixpoint compile (c : cpGCL) : St -> tree St :=
   match c with
   | CSkip => @Leaf _
-  | CAbort => fun st => Fix (fun n => Fail _ n)
+  | CAbort => fun st => Fix (Fail _)
   | CSeq c1 c2 => kcomp (compile c1) (compile c2)
   | CAssign x e => fun st => Leaf (upd x (e st) st)
   | CIte e c1 c2 => fun st => compile (if (e st) then c1 else c2) st
@@ -92,30 +103,69 @@ Fixpoint compile (c : cpGCL) : St -> tree St :=
   end.
 
 
-(** Inference on trees*)
-Fixpoint infer_aux {A : Type} (f : tree A -> Q) (n : nat) (t : tree A) : Q :=
+(** Inference on trees *)
+
+Fixpoint infer_fail {A : Type} (n i : nat) (t : tree A) : Q :=
   match t with
-  | Choice p t1 t2 => p * infer_aux f n t1 + (1-p) * infer_aux f n t2
+  | Leaf _ => 0
+  | Fail _ m => if m =? n then 1 else 0
+  | Choice p t1 t2 => p * infer_fail n i t1 + (1-p) * infer_fail n i t2
   | Fix k =>
-    let a := infer_aux f (S n) (k (S n)) in
-    let b := infer_aux (fun t' => match t' with
-                               | Fail _ m => if Nat.eqb m (S n) then 1 else 0
-                               | _ => 0
-                               end) (S n) (k (S n)) in
+    let a := infer_fail n (S i) (k (S i)) in
+    let b := infer_fail (S i) (S i) (k (S i)) in
     a / (1 - b)
-  | _ => f t
   end.
 
+Fixpoint infer_f {A : Type} (f : A -> Q) (i : nat) (t : tree A) : Q :=
+  match t with
+  | Leaf x => f x
+  | Fail _ _ => 0
+  | Choice p t1 t2 => p * infer_f f i t1 + (1-p) * infer_f f i t2
+  | Fix k =>
+    let a := infer_f f (S i) (k (S i)) in
+    let b := infer_fail (S i) (S i) (k (S i)) in
+    a / (1 - b)
+  end.
+
+
+Fixpoint infer_fail_lib {A : Type} (n i : nat) (t : tree A) : Q :=
+  match t with
+  | Leaf _ => 0
+  | Fail _ m => if m =? n then 1 else 0
+  | Choice p t1 t2 => p * infer_fail n i t1 + (1-p) * infer_fail n i t2
+  | Fix k =>
+    let a := infer_fail_lib n (S i) (k (S i)) in
+    let b := infer_fail_lib (S i) (S i) (k (S i)) in
+    if Qeq_bool b 1 then 1 else a / (1 - b)
+  end.
+
+Fixpoint infer_f_lib {A : Type} (f : A -> Q) (i : nat) (t : tree A) : Q :=
+  match t with
+  | Leaf x => f x
+  | Fail _ _ => 0
+  | Choice p t1 t2 => p * infer_f_lib f i t1 + (1-p) * infer_f_lib f i t2
+  | Fix k =>
+    let a := infer_f_lib f (S i) (k (S i)) in
+    let b := infer_fail_lib (S i) (S i) (k (S i)) in
+    if Qeq_bool b 1 then 1 else a / (1 - b)
+  end.
+  
+
 Definition infer {A : Type} (f : A -> Q) (t : tree A) : Q :=
-  let a := infer_aux (fun t' => match t' with
-                             | Leaf x => f x
-                             | _ => 0
-                             end) O t in
-  let b := infer_aux (fun t' => match t' with
-                             | Fail _ O => 1
-                             | _ => 0
-                             end) O t in
-  a / (1 - b).
+  let a := infer_f f O t in
+  (* let b := infer_fail O O t in *)
+  (* a / (1 - b). *)
+  let b := infer_f_lib (const 1) O t in
+  a / b.
+  (* let b := infer_f (const 1) O t in *)
+  (* a / b. *)
+
+(* Lemma infer_fail_f_lib {A : Type} (f : A -> Q) (t : tree A) (n : nat) : *)
+(*   1 - infer_fail O n t == infer_f_lib (const 1) n t. *)
+(* Proof. *)
+(*   revert f n. induction t; intros f m. *)
+(*   - unfold const; simpl. reflexivity. *)
+(*   - simpl. *)
 
 
 (** Testing inference on example programs *)
@@ -135,6 +185,20 @@ Definition goldfish_piranha_tree : tree St :=
 
 Eval compute in (Qred (infer (fun st => if st O : bool then 1 else 0)
                              goldfish_piranha_tree)).
+
+Definition test_abort : cpGCL :=
+  CChoice (1#3) (CAssign 0%nat (const true)) CAbort.
+
+Definition test_abort_tree : tree St := compile test_abort empty.
+
+Eval compute in (Qred (infer (fun st => if st O : bool then 1 else 0)
+                             test_abort_tree)).
+Eval compute in (Qred (infer (fun st => if negb (st O) then 1 else 0)
+                             test_abort_tree)).
+Eval compute in (Qred (infer (const 1) test_abort_tree)).
+
+Eval compute in (Qred (infer_f (fun st => if st O : bool then 1 else 0) O test_abort_tree)).
+Eval compute in (Qred (infer_f (const 1) O (compile (CChoice (1#2) CSkip CAbort) empty))).
 
 Definition fair_coin : cpGCL :=
   CAssign 0 (const false) ;;
@@ -192,7 +256,7 @@ Inductive wp : cpGCL -> (St -> Q) -> (St -> Q) -> Prop :=
 | wp_while : forall e body f f' ch,
     ch O = const 0 ->
     (forall n, exists g, wp body (ch n) g /\
-               ch (S n) = fun st => if e st : bool then f st else g st) ->
+               ch (S n) = fun st => if e st : bool then g st else f st) ->
     supremum f' ch ->
     wp (CWhile e body) f f'
 | wp_observe : forall e f,
@@ -214,14 +278,15 @@ Inductive wlp : cpGCL -> (St -> Q) -> (St -> Q) -> Prop :=
     wlp c1 f g ->
     wlp c2 f h ->
     wlp (CIte e c1 c2) f (fun st => if e st then g st else h st)
-| wlp_choice : forall p c1 c2 f g h,
+| wlp_choice : forall p c1 c2 f f' g h,
     wlp c1 f g ->
     wlp c2 f h ->
-    wlp (CChoice p c1 c2) f (fun st => p * g st + (1-p) * h st)
+    f' ==f (fun st => p * g st + (1-p) * h st) ->
+    wlp (CChoice p c1 c2) f f'
 | wlp_while : forall e body f f' ch,
     ch O = const 1 ->
     (forall n, exists g, wlp body (ch n) g /\
-               ch (S n) = fun st => if e st : bool then f st else g st) ->
+               ch (S n) ==f fun st => if e st : bool then g st else f st) ->
     infimum f' ch ->
     wlp (CWhile e body) f f'
 | wlp_observe : forall e f,
@@ -233,38 +298,18 @@ Definition cwp_ (c : cpGCL) (f f' g g' : St -> Q) :=
 
 (** cwp is the ratio of the pair given by cwp_ *)
 Definition cwp (c : cpGCL) (f f'' : St -> Q) :=
-  exists f' g', cwp_ c f f' (const 1) g' /\ f'' = fun st => f' st / g' st.
+  exists f' g', cwp_ c f f' (const 1) g' /\ f'' ==f fun st => f' st / g' st.
 
-(* (** Relational specification of CWP semantics *) *)
-(* Inductive cwp_ : cpGCL -> (St -> Q) -> (St -> Q) -> (St -> Q) -> (St -> Q) -> Prop := *)
-(* | cwp_skip : forall f g, cwp_ CSkip f g f g *)
-(* | cwp_assign : forall x e f g, *)
-(*     cwp_ (CAssign x e) f g *)
-(*          (fun st => f (upd x (e st) st)) *)
-(*          (fun st => g (upd x (e st) st)) *)
-(* | cwp_seq : forall c1 c2 f f' f'' g g' g'', *)
-(*     cwp_ c2 f g f' g' -> *)
-(*     cwp_ c1 f' g' f'' g'' -> *)
-(*     cwp_ (CSeq c1 c2) f g f'' g'' *)
-(* | cwp_ite : forall e c1 c2 f f' f'' g g' g'', *)
-(*     cwp_ c1 f g f' g' -> *)
-(*     cwp_ c2 f g f'' g'' -> *)
-(*     cwp_ (CIte e c1 c2) f g *)
-(*          (fun st => if e st then f' st else f'' st) *)
-(*          (fun st => if e st then g' st else g'' st) *)
-(* | cwp_choice : forall p c1 c2 f f' f'' g g' g'', *)
-(*     cwp_ c1 f g f' g' -> *)
-(*     cwp_ c2 f g f'' g'' -> *)
-(*     cwp_ (CChoice p c1 c2) f g *)
-(*          (fun st => p * f' st + (1-p) * f'' st) *)
-(*          (fun st => p * g' st + (1-p) * g'' st) *)
-(* | cwp_while : forall c f g f' g', *)
-(*     lfp f' (fun f_hat => f_hat) -> *)
-(*     cwp_ c f g f' g' *)
-(* | cwp_observe : forall e f g, *)
-(*     cwp_ (CObserve e) f g *)
-(*          (fun st => if e st then f st else 0) *)
-(*          (fun st => if e st then g st else 0). *)
+Ltac wp_inversion :=
+  match goal with
+  | [ H : wp ?c ?f ?f' |- _ ] => inversion H; subst; clear H
+  end.
+
+Ltac wlp_inversion :=
+  match goal with
+  | [ H : wlp ?c ?f ?f' |- _ ] => inversion H; subst; clear H
+  end.
+
 
 (* TODO: restrictions on reading/writing to variables within
    while-loops to ensure correctness of tree inference. *)
@@ -276,116 +321,469 @@ Inductive wf_cpGCL : cpGCL -> Prop :=
     wf_cpGCL c1 -> wf_cpGCL c2 -> wf_cpGCL (CSeq c1 c2)
 | wf_ite : forall e c1 c2,
     wf_cpGCL c1 -> wf_cpGCL c2 -> wf_cpGCL (CIte e c1 c2)
-| wf_choice : forall p c1 c2,
+| wf_cchoice : forall p c1 c2,
     0 <= p <= 1 -> wf_cpGCL c1 -> wf_cpGCL c2 -> wf_cpGCL (CChoice p c1 c2)
 | wf_while : forall e body, wf_cpGCL body -> wf_cpGCL (CWhile e body)
 | wf_observe : forall e, wf_cpGCL (CObserve e).
 
 (** f is an expectation *)
-Definition expectation {A : Type} (f : A -> Q) :=
-  forall x, 0 <= f x.
+Definition expectation {A : Type} (f : A -> Q) := forall x, 0 <= f x.
 
-Lemma Qle_Qdiv_1 (x : Q) :
-  x == x / 1.
+Lemma Qle_Qdiv_1 (x : Q) : x / 1 == x.
 Proof. field. Qed.
 
-(* Maybe decompose this into proofs wrt wp and wlp *)
-Lemma cwp_expectation (c : cpGCL) (f f'' : St -> Q) :
-  expectation f ->
-  cwp c f f'' ->
-  expectation f''.
+Lemma wf_tree_bind {A B : Type} (t : tree A) (k : A -> tree B) :
+  wf_tree t ->
+  (forall x, wf_tree (k x)) ->
+  wf_tree (tree_bind t k).
 Proof.
-  revert f f''.
-  unfold expectation.  
-  induction c; intros f f'' Hexp (f' & g' & [Hcwp0 Hcwp1] & Hcwp2) x.
-  - inversion Hcwp0; subst. inversion Hcwp1; subst.
-    unfold const. specialize (Hexp x).
-    eapply Qle_trans; eauto.
-    rewrite <- Qle_Qdiv_1; apply Qle_refl.
-  - inversion Hcwp0; subst. inversion Hcwp1; subst.
-    unfold const. compute; congruence.
-  - inversion Hcwp0; subst. inversion Hcwp1; subst.
-    unfold const.
-    apply Qle_trans with (y := f (upd n (e x) x)); auto.
-    rewrite <- Qle_Qdiv_1; apply Qle_refl.
-  - inversion Hcwp0; subst. inversion Hcwp1; subst.
-    admit.
-  - admit.
-  - admit.
-  - inversion Hcwp0; subst. inversion Hcwp1; subst.
-    admit.
-  - inversion Hcwp0; subst. inversion Hcwp1; subst.
-    destruct (e x).
-    + eapply Qle_trans; eauto.
-      rewrite <- Qle_Qdiv_1; apply Qle_refl.
-    + compute; congruence.
+  unfold tree_bind. revert k.
+  induction t; intros k Hwf_t Hwf_k; simpl; auto.
+  - constructor.
+  - inversion Hwf_t; subst.
+    constructor; auto.
+  - constructor.
+    intro n. unfold compose.
+    inversion Hwf_t; subst.
+    apply H; auto.
+Qed.
+
+Lemma compile_wf (c : cpGCL) :
+  wf_cpGCL c ->
+  (forall st, wf_tree (compile c st)).
+Proof.
+  induction c; intros Hwf st; try solve [repeat constructor].
+  - inversion Hwf; subst.
+    apply wf_tree_bind; auto.
+  - simpl; inversion Hwf; subst.
+    destruct (e st); auto.
+  - simpl; inversion Hwf; subst.
+    constructor; auto.
+  - simpl. constructor.
+    intro n.
+    inversion Hwf; subst.
+    apply wf_tree_bind; auto.
+    intro x.  destruct (e x); constructor.
+  - simpl. destruct (e st); constructor.
+Qed.
+
+(* Lemma wp_deterministic (c : cpGCL) (f f' f'' : St -> Q) : *)
+(*   wp c f f' -> wp c f f'' -> f' ==f f''. *)
+(* Proof. *)
+(*   revert f f' f''. *)
+(*   induction c; intros f f' f'' Hwp0 Hwp1; *)
+(*     try solve [inversion Hwp0; inversion Hwp1; subst; apply f_Qeq_refl]. *)
+(*   - inversion Hwp0; inversion Hwp1; subst. *)
+(*     (* IH not strong enough for seq case. Need to loosen it to *)
+(*        equivalence of input functions instead of equality.  *) *)
+(* Admitted. *)
+
+(* Lemma wlp_deterministic (c : cpGCL) (f f' f'' : St -> Q) : *)
+(*   wlp c f f' -> wlp c f f'' -> f' ==f f''. *)
+(* Admitted. *)
+
+(* Lemma cwp_deterministic (c : cpGCL) (f f' f'' : St -> Q) : *)
+(*   cwp c f f' -> cwp c f f'' -> f' ==f f''. *)
+(* Admitted. *)
+
+
+(* Lemma jksfdg {A B : Type} (f : B -> Q) (t : nat -> tree A) (k : A -> tree B) (n m : nat) : *)
+(*   infer_f f n (join (fmap k (t m))) = infer_f f (S n) (join (fmap k (t (S n)))). *)
+(* Proof. *)
+(*   revert t k f m. *)
+(*   induction n; intros t k f m. *)
+(*   - simpl. *)
+
+(* Lemma jksfdg {A : Type} (f : A -> Q) (t1 t2 : tree A) (n : nat) : *)
+(*   (* t1 and t2 are alpha equivalent *) *)
+(*   (* all fvs of t1 and t2 are <= n *) *)
+(*   infer_f f n t1 = infer_f f n t2. *)
+(* Proof. *)
+(*   revert t k f m. *)
+(*   induction n; intros t k f m. *)
+(*   - simpl. *)
+
+Lemma infer_f_bind {A B : Type} (f : B -> Q) (t1 : tree A) (k : A -> tree B) (n m : nat) :
+  infer_f (infer_f f n ∘ k) m t1 = infer_f f n (tree_bind t1 k).
+Proof.
+  revert f k n m.
+  induction t1; intros f k m m'; try reflexivity.
+  - simpl in *. rewrite IHt1_1, IHt1_2. reflexivity.
+  - simpl.
+    rewrite H. unfold tree_bind, compose.
+    f_equal.
+    +      
+
+
+      admit.
+    + f_equal.
+      
+    (* unfold tree_bind in H. *)
+    (* unfold compose. *)
+    (* erewrite <- H. *)
+    (* specialize (H (S m') f k m (S m')). *)
+    (* (* unfold tree_bind, compose in H. *) *)
+    (* rewrite H. clear H. *)
+    (* unfold tree_bind. unfold compose. *)
 Admitted.
 
-Lemma wp_deterministic (c : cpGCL) (f f' f'' : St -> Q) :
-  wp c f f' -> wp c f f'' ->
-  f' = f''.
+
+Lemma infer_f_expectation {A : Type} (f : A -> Q) (t : tree A) (n : nat) :
+  wf_tree t ->
+  expectation f ->
+  0 <= infer_f f n t.
 Proof.
-  revert f  f' f''.
-  induction c; intros f f' f'' Hwp0 Hwp1.
-  - inversion Hwp0; subst; inversion Hwp1; subst; reflexivity.
-  - inversion Hwp0; subst; inversion Hwp1; subst; reflexivity.
-  - inversion Hwp0; subst; inversion Hwp1; subst; reflexivity.
-  - inversion Hwp0; subst; inversion Hwp1; subst.
-    eapply IHc2 in H1; eauto; subst.
-    eapply IHc1 in H4; eauto.
-  - inversion Hwp0; subst; inversion Hwp1; subst.
-    eapply IHc1 in H4; eauto; subst.
-    eapply IHc2 in H5; eauto; subst.
-    reflexivity.
-  - inversion Hwp0; subst; inversion Hwp1; subst.
-    eapply IHc1 in H4; eauto; subst.
-    eapply IHc2 in H5; eauto; subst.
-    reflexivity.
-  - 
-    inversion Hwp0; subst; inversion Hwp1; subst.
-    assert (ch = ch0).
+  revert f n. induction t; intros f m Hwf Hexp.
+  - simpl; apply Hexp.
+  - apply Qle_refl.
+  - simpl.
+    inversion Hwf; subst.
+    specialize (IHt1 f m H3 Hexp).
+    specialize (IHt2 f m H4 Hexp).
+    nra.
+  - simpl.
+    inversion Hwf.
+    specialize (H (S m) f (S m) (H1 _) Hexp).
+    assert (infer_fail (S m) (S m) (t (S m)) <= 1).
     { admit. }
     subst.
-    generalize (supremum_unique f' f'' ch0 H5 H8).
-    unfold equ. simpl.
-    intros [Hleq0 Hleq1].
-    extensionality st.
-    admit. (* Need to use Qeq instead of definitional equality -_- *)
-  - inversion Hwp0; subst; inversion Hwp1; subst; reflexivity.
+    assert (0 <= 1 - infer_fail (S m) (S m) (t (S m))).
+    { lra. }
+    apply Qle_lt_or_eq in H0.
+    destruct H0.
+    + apply Qle_shift_div_l; auto; lra.
+    + rewrite <- H0. apply Qle_lteq.
+      right. simpl.
+      admit.
 Admitted.
 
-(* Lemma fair_coin_cwp : *)
-(*   cwp fair_coin (fun st => if st O then 1 else 0) (const (1#2)). *)
 
-(** Probably need to quantify over possible solutions and say that
-    they are equivalent to 1/2 (Qeq).*)
-Lemma fair_coin_cwp :
-  cwp fair_coin (fun st => if st O then 1 else 0) (const (1#2)).
+Theorem wp_infer (c : cpGCL) (f : St -> Q) (n : nat) :
+  wf_cpGCL c ->
+  expectation f ->
+  wp c f (infer_f f n ∘ compile c).
+Proof.
+  revert f n. induction c; intros f m Hwf Hexp; try solve [constructor].
+  (* abort *)
+  - unfold compose. simpl. rewrite Nat.eqb_refl.
+    assert (0 / (1 - 1) = 0).
+    { reflexivity. }
+    rewrite H; constructor.
+    (* sequence *)
+  - unfold compose. simpl.
+    inversion Hwf; subst.
+    specialize (IHc2 f m H2 Hexp).
+    econstructor. apply IHc2; auto.
+    set (f2 := infer_f f m ∘ compile c2).
+    set (f1 := infer_f f2 m ∘ compile c1).
+    set (g := fun x : St => infer_f f m (kcomp (compile c1) (compile c2) x)).
+    (* assert (f1 ==f g). *)
+    (* { intro x; apply infer_f_bind. } *)
+    assert (f1 = g).
+    { extensionality st; apply infer_f_bind. }
+    rewrite <- H.
+    apply IHc1; auto.
+    unfold f2.
+    intro x. unfold compose. 
+    unfold compose in f2. unfold f2.
+    apply infer_f_expectation; auto.
+    apply compile_wf; auto.
+  (* ite *)
+  - unfold compose; simpl.
+    set (fi := infer_f f).
+    assert ((fun x : St => fi m (compile (if e x then c1 else c2) x)) =
+            (fun x => if e x then fi m (compile c1 x) else fi m (compile c2 x))).
+    { extensionality x; destruct (e x); reflexivity. }
+    rewrite H.
+    inversion Hwf; subst.
+    constructor.
+    apply IHc1; auto.
+    apply IHc2; auto.
+  (* choice *)
+  - unfold compose; simpl.
+    inversion Hwf; subst.
+    econstructor.
+    apply IHc1 with (n:=m); auto.
+    apply IHc2 with (n:=m); auto.
+  (* while *)
+  -
+    (* econstructor. *)
+    (* Need to provide a chain of approximations that satisfies the
+       conditions of the while wp constructor, and such that infer
+       after compile yields of the supremum of that chain (probably
+       via an argument based on convergence of geometric series). *)
+    
+    admit.
+  (* observe *)
+  - unfold compose; simpl.
+    assert ((fun x : St =>
+               infer_f f m (if e x then Leaf x else Fail St 0)) =
+            (fun x => if e x then f x else 0)).
+    { extensionality x; destruct (e x); reflexivity. }
+    solve [rewrite H; constructor].
+Admitted.
+
+Theorem wlp_infer (c : cpGCL) (f : St -> Q) (n : nat) :
+  wf_cpGCL c ->
+  expectation f ->
+  wlp c f (fun st => infer_f_lib f n (compile c st)).
+  (* wlp c (const 1) (fun st => 1 - infer_fail O n (compile c st)). *)
+Proof.
+  revert f n. induction c; intros f m Hwf Hexp; try solve [constructor].
+  (* abort *)
+  - simpl; rewrite Nat.eqb_refl; constructor.
+  (* sequence *)
+  - simpl.
+    inversion Hwf; subst.
+    econstructor.
+    apply IHc2 with (n:=m); auto.
+    assert (Hexp': expectation ((fun st : St => infer_f_lib f m (compile c2 st)))).
+    { admit. }
+    specialize (IHc1 _ m H1 Hexp').
+    assert (Heq: (fun st : St => infer_f_lib
+                                f m (kcomp (compile c1) (compile c2) st)) =
+                 (fun st : St =>
+                    infer_f_lib
+                      (fun st0 : St => infer_f_lib f m (compile c2 st0))
+                      m (compile c1 st))).
+    { extensionality st. admit. }
+    solve [rewrite Heq; apply IHc1].
+  (* ite *)
+  - simpl.
+    assert (Heq: (fun st : St => infer_f_lib
+                                f m (compile (if e st then c1 else c2) st)) =
+                 (fun st : St => if e st
+                              then infer_f_lib f m (compile c1 st)
+                              else infer_f_lib f m (compile c2 st))).
+    { extensionality x; destruct (e x); reflexivity. }
+    rewrite Heq.
+    inversion Hwf; subst.
+    constructor; auto.
+  (* choice *)
+  - simpl; inversion Hwf; subst.
+    econstructor.
+    apply IHc1 with (n:=m); auto.
+    apply IHc2 with (n:=m); auto.
+    intro st; simpl; field.
+  (* while *)
+  - admit.
+  (* observe *)
+  - simpl.
+    assert (Heq: (fun st : St =>
+                    infer_f_lib f m (if e st then Leaf st else Fail St 0)) =
+                 fun st => if e st then f st else 0).
+    { extensionality st; destruct (e st); reflexivity. }
+    rewrite Heq; constructor.
+Admitted.
+
+Theorem infer_correct (c : cpGCL) (f : St -> Q) :
+  wf_cpGCL c ->
+  expectation f ->
+  cwp c f (infer f ∘ compile c).
+Proof.
+  intros Hwf Hexp.
+  eexists. eexists. split.
+  - split.
+    + apply wp_infer with (n:=O); auto.
+    + apply wlp_infer with (n:=O); auto.
+      compute; congruence.
+  - reflexivity.
+Qed.
+
+
+(** Using CWP on example programs *)
+
+Lemma goldfish_piranha_cwp (f : St -> Q) :
+  cwp goldfish_piranha (fun st => if st O then 1 else 0) f -> f ==f const (2#3).
+Proof.
+  unfold goldfish_piranha, cwp.
+  intros (f' & g' & [Hwp Hwlp] & Hf).
+  repeat wp_inversion; repeat wlp_inversion.
+  simpl in *; unfold const in *.
+  intro x; rewrite Hf; rewrite H8; rewrite 2!H9.
+  compute; reflexivity.
+Qed.
+
+Fixpoint Qpow (x : Q) (n : nat) :=
+  match n with
+  | O => 1
+  | S n' => x * Qpow x n'
+  end.
+
+Fixpoint geometric_series (a r : Q) (n : nat) :=
+  match n with
+  | O => a
+  | S n' => geometric_series a r n' + a * Qpow r n
+  end.
+
+(* Eval compute in (Qred (geometric_series (2#9) (5#9) 10)). *)
+
+Axiom geometric_series_converges :
+  forall a r eps,
+    0 <= a <= 1 -> 0 <= r -> r < 1 -> 0 < eps ->
+    exists n0, forall n,
+        (n0 <= n)%nat -> (a / (1 - r)) - geometric_series a r n < eps.
+
+Lemma geometric_series_fact (a r : Q) (n : nat) :
+  a + r * geometric_series a r n == geometric_series a r (S n).
+Proof.
+  induction n.
+  - simpl; field.
+  - rewrite <- IHn.
+Admitted.
+
+Lemma fair_coin_cwp (f : St -> Q) :
+  cwp fair_coin (fun st => if st O then 1 else 0) f -> f ==f const (1#2).
 Proof.
   unfold fair_coin.
   unfold cwp.
-  eexists. eexists.
-  unfold cwp_. split. split.
-  - econstructor.
-    + econstructor.
-      * admit.
-      * econstructor.
-    + econstructor.
-  - econstructor.
-    + econstructor.
-      * admit.
-      * econstructor.
-    + econstructor.
-  - 
-    extensionality st. unfold const.
-    admit.
-Admitted.
+  intros (f' & g' & [Hwp Hwlp] & Hf).
+  set (fx := fun st : St => if st O : bool then 1 else 0).
+  repeat wp_inversion.
+  repeat wlp_inversion.  
+  intro x. rewrite Hf. unfold const.
 
+  assert (forall i, ch0 i ==f const 1).
+  { clear Hf. clear H3. clear H6. clear H1. clear ch.
+    clear H9. clear x. clear f f' f'1.
+    intro i. induction i.
+    - intro x; rewrite H2; reflexivity.
+    - specialize (H5 i).
+      destruct H5 as (g & Hwlp & H).
+      repeat wlp_inversion.
+      unfold const in *.
+      intro st.
+      assert (H9' := H9).
+      specialize (H9 (upd O true st)).
+      specialize (H9' (upd O false st)).
+      specialize (H10 st).
+      rewrite 2!IHi in H9.
+      rewrite 2!IHi in H9'.
+      rewrite H9 in H10.
+      rewrite H9' in H10.
+      rewrite H.
+      destruct (eqb (st O) (st (S O))); try reflexivity.
+      rewrite H10. field. }
 
-(** Main theorem establishing correctness of compilation+inference
-    wrt. CWP semantics. *)
-Theorem cwp_infer (c : cpGCL) (f f' : St -> Q) :
-  wf_cpGCL c ->
-  expectation f ->
-  cwp c f f' <-> forall st, infer f (compile c st) == f' st.
-Admitted.
+  assert (infimum (const 1) ch0).
+  { apply const_infimum; intro i; apply f_Qeq_equ; auto. }
+  assert (Hf'1: f'1 ==f const 1).
+  { apply f_Qeq_equ; eapply infimum_unique; eauto. }
+  rewrite Hf'1.
+
+  assert (supremum (fun st => if eqb (st O) (st (S O)) then 1#2 else fx st) ch).
+  {
+    split.
+    - intros i st. unfold const; simpl.
+      clear Hf. clear H6. clear H2. clear H5. clear H9.
+      clear x. clear H0. clear Hf'1. clear H.
+      clear ch0. revert st.
+      induction i; intro st.
+      + rewrite H1. unfold const, fx.
+        destruct (st O); destruct (st (S O)); simpl; compute; congruence.
+      + specialize (H3 i).
+        destruct H3 as (g & Hwp & H).
+        repeat wp_inversion.
+        unfold const in H.
+        rewrite H.
+        assert (Hi0 := IHi (upd 1 true (upd 0 true st))).
+        assert (Hi1 := IHi (upd 1 false (upd 0 true st))).
+        assert (Hi2 := IHi (upd 1 true (upd 0 false st))).
+        assert (Hi3 := IHi (upd 1 false (upd 0 false st))).
+        unfold fx in *. simpl in *.
+        destruct (st O) eqn:Hx; destruct (st (S O)) eqn:Hy; simpl in *; try lra.
+    - intros ub Hub st.
+      unfold upper_bound in Hub.
+      simpl in *.
+      unfold fx.
+
+      assert (forall i, ch (S (S i)) ==f fun st => if eqb (st O) (st (S O))
+                                           then geometric_series (2#9) (5#9) i
+                                           else fx st).
+      { clear Hf. clear H6. clear H2. clear H5. clear H9.
+        clear x. clear H0. clear Hf'1. clear H.
+        clear ch0. revert st.
+        clear Hub ub.
+        induction i; intro x.
+        - simpl.
+          assert (Hch1 := H3 O).
+          specialize (H3 (S O)).
+          destruct H3 as (g & Hwp & H3).
+          rewrite H3.
+          simpl.
+          repeat wp_inversion.          
+          destruct Hch1 as (g & Hwp & Hch1).
+          repeat wp_inversion.
+          unfold const in *.
+          rewrite Hch1. unfold fx. simpl. rewrite H1.
+          destruct (x O); destruct (x (S O)); reflexivity.
+        - set (geom := geometric_series (2#9) (5#9) (S i)).
+          simpl.
+          destruct (H3 (S (S i))) as (g & Hwp & Hch).
+          repeat wp_inversion.
+          rewrite Hch. unfold const.
+          clear Hch.
+          unfold fx in *.
+          destruct (x O); destruct (x (S O)); simpl; try rewrite 4!IHi; simpl.
+          + unfold geom. rewrite <- geometric_series_fact. simpl. field.
+          + reflexivity.
+          + reflexivity.
+          + simpl.
+            unfold geom. rewrite <- geometric_series_fact. field. }
+
+      assert (Hle0: 0 <= 2#9 <= 1). lra.
+      assert (Hle1: 0 <= 5#9). lra.
+      assert (Hlt: 5#9 < 1). lra.
+      destruct (st O) eqn:Hx; destruct (st (S O)) eqn:Hy; simpl.
+      + assert (forall eps, 0 < eps -> exists n0, (1#2) - ch n0 st < eps).
+        { intros eps Heps.
+          generalize (@geometric_series_converges _ _ _ Hle0 Hle1 Hlt Heps).
+          intros [n0 Hgeom].
+          exists (S (S n0)).
+          rewrite H4.
+          rewrite Hx. rewrite Hy. simpl.
+          specialize (Hgeom n0 (Nat.le_refl _)).
+          assert (H7: (2#9) / (1 - (5#9)) == 1#2).
+          { reflexivity. }
+          rewrite <- H7. apply Hgeom. }
+        destruct (Qlt_le_dec (ub st) (1#2)); auto.
+        * assert (0 < (1#2) - ub st).
+          { lra. }
+          specialize (H7 ((1#2) - ub st) H8).
+          destruct H7 as [n0 H7].
+          assert (ub st < ch n0 st).
+          { lra. }
+          specialize (Hub n0 st).
+          lra.
+      + specialize (Hub (S O) st).
+        specialize (H3 O).
+        destruct H3 as (g & Hwp & H3).
+        rewrite H3 in Hub.
+        rewrite Hx in Hub.
+        rewrite Hy in Hub.
+        apply Hub.
+      + specialize (Hub O st). rewrite H1 in Hub. apply Hub.
+      + assert (forall eps, 0 < eps -> exists n0, (1#2) - ch n0 st < eps).
+        { intros eps Heps.
+          generalize (@geometric_series_converges _ _ _ Hle0 Hle1 Hlt Heps).
+          intros [n0 Hgeom].
+          exists (S (S n0)).
+          rewrite H4.
+          rewrite Hx. rewrite Hy. simpl.
+          specialize (Hgeom n0 (Nat.le_refl _)).
+          assert (H7: (2#9) / (1 - (5#9)) == 1#2).
+          { reflexivity. }
+          rewrite <- H7. apply Hgeom. }
+        destruct (Qlt_le_dec (ub st) (1#2)); auto.
+        * assert (0 < (1#2) - ub st).
+          { lra. }
+          specialize (H7 ((1#2) - ub st) H8).
+          destruct H7 as [n0 H7].
+          assert (ub st < ch n0 st).
+          { lra. }
+          specialize (Hub n0 st).
+          lra. }
+  assert (Hf' : f' ==f fun st => if eqb (st O) (st (S O)) then 1#2 else fx st).
+  { apply f_Qeq_equ; eapply supremum_unique; eauto. }
+  rewrite Hf'; reflexivity.
+Qed.
